@prefix : <https://www.w3id.org/statbarnsdc#> .
@prefix owl: <http://www.w3.org/2002/07/owl#> .
@prefix rdf: <http://www.w3.org/1999/02/22-rdf-syntax-ns#> .
@prefix sdc: <https://www.w3id.org/statbarnsdc> .
@prefix xml: <http://www.w3.org/XML/1998/namespace> .
@prefix xsd: <http://www.w3.org/2001/XMLSchema#> .
@prefix dcam: <http://purl.org/dc/dcam/> .
@prefix foaf: <http://xmlns.com/foaf/0.1/> .
@prefix rdfs: <http://www.w3.org/2000/01/rdf-schema#> .
@prefix skos: <http://www.w3.org/2004/02/skos/core#> .
@prefix vann: <http://purl.org/vocab/vann/> .
@prefix schema: <https://schema.org/> .
@prefix dcterms: <http://purl.org/dc/terms/> .
@prefix dpv-owl: <https://w3id.org/dpv/owl#> .
@prefix risk-owl: <https://w3id.org/dpv/risk/owl#> .
@base <https://www.w3id.org/statbarnsdc#> .

<https://www.w3id.org/statbarnsdc> rdf:type owl:Ontology ;
                                    owl:versionIRI <https://www.w3id.org/statbarnsdc/1.0> ;
                                    owl:imports <https://w3id.org/dpv/2.2/owl#> ,
                                                <https://w3id.org/dpv/2.2/risk/owl#> ;
                                    dcterms:creator "Trupti Padiya - University of the West of England (UWE Bristol), ORCID:0000-0003-4514-4473 " ;
                                    dcterms:contributor "Jim Smith - University of the West of England (UWE Bristol), ORCID:0000-0001-7908-1859 " ,
                                                        "Felix Ritchie - University of the West of England (UWE Bristol), ORCID:0000-0003-4097-4021" ,
                                                        "Elizabeth Green - University of the West of England (UWE Bristol), ORCID: 0000-0002-5199-9534" ,
                                                        "Amy Tilbrook - University of Edinburgh, Health Data Research UK, ORCID:0000-0002-0294-2101" ;
                                    dcterms:description "An Ontology for the Statbarn Framework used in Output Statistical Disclosure Control (OSDC)." ;
                                    dcterms:license <https://opensource.org/licenses/MIT> ;
                                    dcterms:title "StatbarnSDC Ontology" ;
                                    vann:preferredNamespacePrefix "sdc" ;
                                    skos:scopeNote "The concepts described in the ontology are in accordance with the Statbarn framework used in Output Statistical Disclosure Control." .

#################################################################
#    Data properties
#################################################################

###  https://www.w3id.org/statbarnsdc#hasBooleanValue
:hasBooleanValue rdf:type owl:DatatypeProperty ;
                 rdfs:range xsd:boolean ;
                 rdfs:isDefinedBy "https://www.w3id.org/statbarnsdc" ;
                 skos:definition "Indicates a boolean value" ;
                 skos:prefLabel "hasBooleanValue" .


###  https://www.w3id.org/statbarnsdc#hasDecimalValue
:hasDecimalValue rdf:type owl:DatatypeProperty ;
                 rdfs:range xsd:decimal ;
                 rdfs:isDefinedBy "https://www.w3id.org/statbarnsdc" ;
                 skos:definition "Indicates a decimal value" ;
                 skos:prefLabel "hasDecimalValue" .


#################################################################
#    Classes
#################################################################

###  https://www.w3id.org/statbarnsdc#AdditiveNoise
:AdditiveNoise rdf:type owl:Class ;
               rdfs:subClassOf :Noise ;
               rdfs:isDefinedBy "https://www.w3id.org/statbarnsdc" ;
               skos:definition "Random values are added to original data to obscure individual contributions to control disclosure risk." ;
               skos:prefLabel "AdditiveNoise" .


###  https://www.w3id.org/statbarnsdc#AdjustedRSquared
:AdjustedRSquared rdf:type owl:Class ;
                  rdfs:subClassOf :StatisticalHypothesisTests ;
                  rdfs:isDefinedBy "https://www.w3id.org/statbarnsdc" ;
                  skos:definition "A statistical measure that indicates how well a regression model explains the variability of the dependent variable." ;
                  skos:prefLabel "AdjustedRSquared" .


###  https://www.w3id.org/statbarnsdc#Aggregation
:Aggregation rdf:type owl:Class ;
             rdfs:subClassOf risk-owl:MitigationControl ;
             rdfs:isDefinedBy "https://www.w3id.org/statbarnsdc" ;
             skos:definition "A risk mitigation technique where individual data are combined into larger groups or summaries to reduce the risk of identifying or inferring information about specific individuals." ;
             skos:prefLabel "Aggregation" .


###  https://www.w3id.org/statbarnsdc#AlluvialFlow
:AlluvialFlow rdf:type owl:Class ;
              rdfs:subClassOf :Frequencies ;
              rdfs:isDefinedBy "https://www.w3id.org/statbarnsdc" ;
              skos:definition "A type of diagram that visualizes changes in categorical data over time or between stages, showing how groups split, merge, or flow from one category to another." ;
              skos:prefLabel "AlluvialFlow" .


###  https://www.w3id.org/statbarnsdc#AnalysisOfVariance
:AnalysisOfVariance rdf:type owl:Class ;
                    rdfs:subClassOf :StatisticalHypothesisTests ;
                    rdfs:isDefinedBy "https://www.w3id.org/statbarnsdc" ;
                    skos:definition "Also reffered to as ANOVA is a statistical method used to compare the means of three or more groups." ;
                    skos:prefLabel "AnalysisOfVariance" .


###  https://www.w3id.org/statbarnsdc#Ancova
:Ancova rdf:type owl:Class ;
        rdfs:subClassOf :CorrelationCoefficients ;
        rdfs:isDefinedBy "https://www.w3id.org/statbarnsdc" ;
        skos:definition "Combines ANOVA and regression to compare group means while controlling for one or more continuous covariates." ;
        skos:prefLabel "Ancova" .


###  https://www.w3id.org/statbarnsdc#AuxiliaryInformation
:AuxiliaryInformation rdf:type owl:Class ;
                      rdfs:subClassOf dpv-owl:Risk ,
                                      [ rdf:type owl:Restriction ;
                                        owl:onProperty risk-owl:hasRiskEvaluation ;
                                        owl:someValuesFrom :StatbarnDataCheck
                                      ] ,
                                      [ rdf:type owl:Restriction ;
                                        owl:onProperty dpv-owl:hasLikelihood ;
                                        owl:allValuesFrom dpv-owl:Likelihood
                                      ] ,
                                      [ rdf:type owl:Restriction ;
                                        owl:onProperty dpv-owl:hasRiskLevel ;
                                        owl:allValuesFrom dpv-owl:RiskLevel
                                      ] ;
                      rdfs:isDefinedBy "https://www.w3id.org/statbarnsdc" ;
                      skos:definition "The risk that external data, when combined with published statistical outputs, will allow inferences or identification of individuals, increasing disclosure risk beyond what the output alone suggests." ;
                      skos:prefLabel "AuxiliaryInformation" .


###  https://www.w3id.org/statbarnsdc#BarGraph
:BarGraph rdf:type owl:Class ;
          rdfs:subClassOf :LinearAggregations ;
          rdfs:isDefinedBy "https://www.w3id.org/statbarnsdc" ;
          skos:definition "A chart that represents categorical data with rectangular bars, where the length of each bar is proportional to the value or frequency of the category." ;
          skos:prefLabel "BarGraph" .


###  https://www.w3id.org/statbarnsdc#BartlettsTestOfSphericity
:BartlettsTestOfSphericity rdf:type owl:Class ;
                           rdfs:subClassOf :StatisticalHypothesisTests ;
                           rdfs:isDefinedBy "https://www.w3id.org/statbarnsdc" ;
                           skos:definition "A statistical test used to check whether a correlation matrix is an identity matrix." ;
                           skos:prefLabel "BartlettsTestOfSphericity" .


###  https://www.w3id.org/statbarnsdc#BetaCoefficient
:BetaCoefficient rdf:type owl:Class ;
                 rdfs:subClassOf :LinearAggregations ;
                 rdfs:isDefinedBy "https://www.w3id.org/statbarnsdc" ;
                 skos:definition "A standardized regression coefficient that indicates the strength and direction of the relationship between a predictor and the outcome." ;
                 skos:prefLabel "BetaCoefficient" .


###  https://www.w3id.org/statbarnsdc#BinaryLogisticRegression
:BinaryLogisticRegression rdf:type owl:Class ;
                          rdfs:subClassOf :CorrelationCoefficients ;
                          rdfs:isDefinedBy "https://www.w3id.org/statbarnsdc" ;
                          skos:definition "A statistical model used to predict the probability of a binary outcome." ;
                          skos:prefLabel "BinaryLogisticRegression" .


###  https://www.w3id.org/statbarnsdc#BoxPlot
:BoxPlot rdf:type owl:Class ;
         rdfs:subClassOf :Position ;
         rdfs:isDefinedBy "https://www.w3id.org/statbarnsdc" ;
         skos:definition "A graphical display that summarizes the distribution of a dataset using its minimum, first quartile, median, third quartile, and maximum, often highlighting outliers." ;
         skos:prefLabel "BoxPlot" .


###  https://www.w3id.org/statbarnsdc#BoxsTestOfEqualityOfCovarianceMatrices
:BoxsTestOfEqualityOfCovarianceMatrices rdf:type owl:Class ;
                                        rdfs:subClassOf :StatisticalHypothesisTests ;
                                        rdfs:isDefinedBy "https://www.w3id.org/statbarnsdc" ;
                                        skos:definition "Statistical test used to assess whether the covariance matrices of multiple groups are equal." ;
                                        skos:prefLabel "BoxsTestOfEqualityOfCovarianceMatrices" .


###  https://www.w3id.org/statbarnsdc#CalculatedRatios
:CalculatedRatios rdf:type owl:Class ;
                  rdfs:subClassOf :Statbarn ,
                                  [ rdf:type owl:Restriction ;
                                    owl:onProperty dpv-owl:hasRisk ;
                                    owl:someValuesFrom :AuxiliaryInformation
                                  ] ,
                                  [ rdf:type owl:Restriction ;
                                    owl:onProperty dpv-owl:hasRisk ;
                                    owl:someValuesFrom :Dominance
                                  ] ;
                  rdfs:isDefinedBy "https://www.w3id.org/statbarnsdc" ;
                  skos:definition "Calculated ratios refer to measures investigating relationship, comparison or relative magnitude between variables. These can includes odds ratios, risk ratios, or hazard ratios." ;
                  skos:prefLabel "CalculatedRatios" .


###  https://www.w3id.org/statbarnsdc#CanonicalCorrelation
:CanonicalCorrelation rdf:type owl:Class ;
                      rdfs:subClassOf :CorrelationCoefficients ;
                      rdfs:isDefinedBy "https://www.w3id.org/statbarnsdc" ;
                      skos:definition "Measures the relationship between two sets of variables." ;
                      skos:prefLabel "CanonicalCorrelation" .


###  https://www.w3id.org/statbarnsdc#CategoricalAggregation
:CategoricalAggregation rdf:type owl:Class ;
                        rdfs:subClassOf :Aggregation ;
                        rdfs:isDefinedBy "https://www.w3id.org/statbarnsdc" ;
                        skos:definition "Combining categories of a categorical variable to reduce the granularity of the data to reduce disclosure risk." ;
                        skos:prefLabel "CategoricalAggregation" .


###  https://www.w3id.org/statbarnsdc#CellKeyRounding
:CellKeyRounding rdf:type owl:Class ;
                 rdfs:subClassOf :Rounding ;
                 rdfs:isDefinedBy "https://www.w3id.org/statbarnsdc" ;
                 skos:definition "Cell values in tables are rounded based on a key or algorithm to reduce risk." ;
                 skos:prefLabel "CellKeyRounding" .


###  https://www.w3id.org/statbarnsdc#ChiSquaredTest
:ChiSquaredTest rdf:type owl:Class ;
                rdfs:subClassOf :StatisticalHypothesisTests ;
                rdfs:isDefinedBy "https://www.w3id.org/statbarnsdc" ;
                skos:definition "Statistical test used to determine whether there is a significant association between categorical variables." ;
                skos:prefLabel "ChiSquaredTest" .


###  https://www.w3id.org/statbarnsdc#ClassDisclosure
:ClassDisclosure rdf:type owl:Class ;
                 rdfs:subClassOf dpv-owl:Risk ,
                                 [ rdf:type owl:Restriction ;
                                   owl:onProperty risk-owl:hasRiskEvaluation ;
                                   owl:someValuesFrom :RequiredZeroCheck
                                 ] ,
                                 [ rdf:type owl:Restriction ;
                                   owl:onProperty dpv-owl:hasLikelihood ;
                                   owl:allValuesFrom dpv-owl:Likelihood
                                 ] ,
                                 [ rdf:type owl:Restriction ;
                                   owl:onProperty dpv-owl:isMitigatedByMeasure ;
                                   owl:allValuesFrom [ rdf:type owl:Class ;
                                                       owl:unionOf ( :Noise
                                                                     :Suppression
                                                                   )
                                                     ]
                                 ] ,
                                 [ rdf:type owl:Restriction ;
                                   owl:onProperty risk-owl:hasRiskEvaluation ;
                                   owl:allValuesFrom :PresenceOfZeroCheck
                                 ] ;
                 rdfs:isDefinedBy "https://www.w3id.org/statbarnsdc" ;
                 skos:definition "The risk that released statistical outputs allow an attacker to infer details about an individual, as a result of their membership of a sensitive category or class who all share the same values  for some variables." ;
                 skos:prefLabel "ClassDisclosure" .


###  https://www.w3id.org/statbarnsdc#Clusters
:Clusters rdf:type owl:Class ;
          rdfs:subClassOf :Statbarn ;
          rdfs:isDefinedBy "https://www.w3id.org/statbarnsdc" ;
          skos:definition "Statbarn classification that covers output of cluster analysis. Cluster analysis is a statistical technique used to classify or group similar objects or individuals based on their characteristics or attributes. It aims to identify patterns, similarities, or relationships within a dataset by grouping data points into clusters." ;
          skos:prefLabel "Clusters" .


###  https://www.w3id.org/statbarnsdc#CochransQTest
:CochransQTest rdf:type owl:Class ;
               rdfs:subClassOf :StatisticalHypothesisTests ;
               rdfs:isDefinedBy "https://www.w3id.org/statbarnsdc" ;
               skos:definition "Statistical test used to determine whether there are differences in proportions across three or more related groups for binary outcomes." ;
               skos:prefLabel "CochransQTest" .


###  https://www.w3id.org/statbarnsdc#CoefficientOfDetermination
:CoefficientOfDetermination rdf:type owl:Class ;
                            rdfs:subClassOf :StatisticalHypothesisTests ;
                            rdfs:isDefinedBy "https://www.w3id.org/statbarnsdc" ;
                            skos:definition "Statistical measure that indicates the proportion of variance in the dependent variable explained by the independent variable(s) in a regression model." ;
                            skos:prefLabel "CoefficientOfDetermination" .


###  https://www.w3id.org/statbarnsdc#CohensD
:CohensD rdf:type owl:Class ;
         rdfs:subClassOf :StatisticalHypothesisTests ;
         rdfs:isDefinedBy "https://www.w3id.org/statbarnsdc" ;
         skos:definition "Measure of effect size that quantifies the difference between two group means in terms of standard deviation units." ;
         skos:prefLabel "CohensD" .


###  https://www.w3id.org/statbarnsdc#CohensKappaCoefficient
:CohensKappaCoefficient rdf:type owl:Class ;
                        rdfs:subClassOf :StatisticalHypothesisTests ;
                        rdfs:isDefinedBy "https://www.w3id.org/statbarnsdc" ;
                        skos:definition "Measures the level of agreement between two raters or observers for categorical data, adjusting for agreement occurring by chance." ;
                        skos:prefLabel "CohensKappaCoefficient" .


###  https://www.w3id.org/statbarnsdc#ConfidenceIntervals
:ConfidenceIntervals rdf:type owl:Class ;
                     rdfs:subClassOf :StatisticalHypothesisTests ;
                     rdfs:isDefinedBy "https://www.w3id.org/statbarnsdc" ;
                     skos:definition "Range of values, derived from sample data, that likely contain the true population parameter with a specified level of confidence." ;
                     skos:prefLabel "ConfidenceIntervals" .


###  https://www.w3id.org/statbarnsdc#ContrastCoefficients
:ContrastCoefficients rdf:type owl:Class ;
                      rdfs:subClassOf :CorrelationCoefficients ;
                      rdfs:isDefinedBy "https://www.w3id.org/statbarnsdc" ;
                      skos:definition "Numerical weights assigned to group means in ANOVA or regression." ;
                      skos:prefLabel "ContrastCoefficients" .


###  https://www.w3id.org/statbarnsdc#ControlledRounding
:ControlledRounding rdf:type owl:Class ;
                    rdfs:subClassOf :Rounding ;
                    rdfs:isDefinedBy "https://www.w3id.org/statbarnsdc" ;
                    skos:definition "Table or cell values are rounded according to specific rules to prevent disclosure risk." ;
                    skos:prefLabel "ControlledRounding" .


###  https://www.w3id.org/statbarnsdc#CorrelationCoefficients
:CorrelationCoefficients rdf:type owl:Class ;
                         rdfs:subClassOf :Statbarn ,
                                         [ rdf:type owl:Restriction ;
                                           owl:onProperty dpv-owl:hasRisk ;
                                           owl:someValuesFrom :LowDOF
                                         ] ;
                         rdfs:isDefinedBy "https://www.w3id.org/statbarnsdc" ;
                         skos:definition "Correlation coefficients are statistical measures that quantify the relationship between two or more variables. This includes measures such as regression estimates, as well as single statistics such as Pearson's r, Spearmans's rank correlation coefficient (ρ) and Kendall's rank correlation coefficient (τ)." ;
                         skos:prefLabel "CorrelationCoefficients" .


###  https://www.w3id.org/statbarnsdc#Covariates
:Covariates rdf:type owl:Class ;
            rdfs:subClassOf :CorrelationCoefficients ;
            rdfs:isDefinedBy "https://www.w3id.org/statbarnsdc" ;
            skos:definition "Continuous or categorical variables that are included in a statistical model to account for or control their effect on the outcome variable." ;
            skos:prefLabel "Covariates" .


###  https://www.w3id.org/statbarnsdc#CoxSnellRSquared
:CoxSnellRSquared rdf:type owl:Class ;
                  rdfs:subClassOf :StatisticalHypothesisTests ;
                  rdfs:isDefinedBy "https://www.w3id.org/statbarnsdc" ;
                  skos:definition "Measure of goodness-of-fit for logistic regression models." ;
                  skos:prefLabel "CoxSnellRSquared" .


###  https://www.w3id.org/statbarnsdc#CramersV
:CramersV rdf:type owl:Class ;
          rdfs:subClassOf :StatisticalHypothesisTests ;
          rdfs:isDefinedBy "https://www.w3id.org/statbarnsdc" ;
          skos:definition "Measure of association between two categorical variables." ;
          skos:prefLabel "CramersV" .


###  https://www.w3id.org/statbarnsdc#Crosstabs
:Crosstabs rdf:type owl:Class ;
           rdfs:subClassOf :Frequencies ;
           rdfs:isDefinedBy "https://www.w3id.org/statbarnsdc" ;
           skos:definition "A tabular method for displaying the frequency distribution of two or more categorical variables." ;
           skos:prefLabel "Crosstabs" .


###  https://www.w3id.org/statbarnsdc#Differencing
:Differencing rdf:type owl:Class ;
              rdfs:subClassOf dpv-owl:Risk ,
                              [ rdf:type owl:Restriction ;
                                owl:onProperty risk-owl:hasRiskEvaluation ;
                                owl:someValuesFrom :PresenceOfLinkedTableCheck
                              ] ,
                              [ rdf:type owl:Restriction ;
                                owl:onProperty dpv-owl:hasLikelihood ;
                                owl:allValuesFrom dpv-owl:Likelihood
                              ] ,
                              [ rdf:type owl:Restriction ;
                                owl:onProperty dpv-owl:isMitigatedByMeasure ;
                                owl:allValuesFrom [ rdf:type owl:Class ;
                                                    owl:unionOf ( :Noise
                                                                  :Suppression
                                                                )
                                                  ]
                              ] ;
              rdfs:isDefinedBy "https://www.w3id.org/statbarnsdc" ;
              skos:definition "A risk that combining multiple outputs allows to deduce sensitive information about individuals by analyzing changes or differences between them." ;
              skos:prefLabel "Differencing" .


###  https://www.w3id.org/statbarnsdc#DiscriminantFunctionAnalysis
:DiscriminantFunctionAnalysis rdf:type owl:Class ;
                              rdfs:subClassOf :StatisticalHypothesisTests ;
                              rdfs:isDefinedBy "https://www.w3id.org/statbarnsdc" ;
                              skos:definition "Statistical technique used to classify observations into predefined groups and determine which variables best separate those groups." ;
                              skos:prefLabel "DiscriminantFunctionAnalysis" .


###  https://www.w3id.org/statbarnsdc#DiscriminantValidity
:DiscriminantValidity rdf:type owl:Class ;
                      rdfs:subClassOf :StatisticalHypothesisTests ;
                      rdfs:isDefinedBy "https://www.w3id.org/statbarnsdc" ;
                      skos:definition "Extent to which a construct or measurement is truly distinct from other constructs, showing it measures what it is intended to and not something else." ;
                      skos:prefLabel "DiscriminantValidity" .


###  https://www.w3id.org/statbarnsdc#Dominance
:Dominance rdf:type owl:Class ;
           rdfs:subClassOf dpv-owl:Risk ,
                           [ rdf:type owl:Restriction ;
                             owl:onProperty risk-owl:hasRiskEvaluation ;
                             owl:someValuesFrom :NKCheck
                           ] ,
                           [ rdf:type owl:Restriction ;
                             owl:onProperty risk-owl:hasRiskEvaluation ;
                             owl:someValuesFrom :PQCheck
                           ] ,
                           [ rdf:type owl:Restriction ;
                             owl:onProperty dpv-owl:hasLikelihood ;
                             owl:allValuesFrom dpv-owl:Likelihood
                           ] ,
                           [ rdf:type owl:Restriction ;
                             owl:onProperty dpv-owl:isMitigatedByMeasure ;
                             owl:allValuesFrom [ rdf:type owl:Class ;
                                                 owl:unionOf ( :Noise
                                                               :OutlierRemoval
                                                               :Rounding
                                                               :Suppression
                                                             )
                                               ]
                           ] ;
           rdfs:isDefinedBy "https://www.w3id.org/statbarnsdc" ;
           skos:definition "The risk that a small number of individuals contribute a disproportionately large share of a cells value, making it easier to identify or infer their data." ;
           skos:prefLabel "Dominance" .


###  https://www.w3id.org/statbarnsdc#EigenvaluesScreePlots
:EigenvaluesScreePlots rdf:type owl:Class ;
                       rdfs:subClassOf :StatisticalHypothesisTests ;
                       rdfs:isDefinedBy "https://www.w3id.org/statbarnsdc" ;
                       skos:definition "Eigenvalues measure the amount of variance explained by each factor, and a scree plot visualizes these values to help decide how many factors to retain." ;
                       skos:prefLabel "EigenvaluesScreePlots" .


###  https://www.w3id.org/statbarnsdc#Endpoints
:Endpoints rdf:type owl:Class ;
           rdfs:subClassOf :Statbarn ,
                           [ rdf:type owl:Restriction ;
                             owl:onProperty dpv-owl:hasRisk ;
                             owl:someValuesFrom :ClassDisclosure
                           ] ,
                           [ rdf:type owl:Restriction ;
                             owl:onProperty dpv-owl:hasRisk ;
                             owl:someValuesFrom :LowCount
                           ] ;
           rdfs:isDefinedBy "https://www.w3id.org/statbarnsdc" ;
           skos:definition "Minimum and maximum values for a variable." ;
           skos:prefLabel "Endpoints" .


###  https://www.w3id.org/statbarnsdc#EtaSquared
:EtaSquared rdf:type owl:Class ;
            rdfs:subClassOf :StatisticalHypothesisTests ;
            rdfs:isDefinedBy "https://www.w3id.org/statbarnsdc" ;
            skos:definition "Measure of effect size that indicates the proportion of total variance in a dependent variable explained by an independent variable in ANOVA or similar analyses." ;
            skos:prefLabel "EtaSquared" .


###  https://www.w3id.org/statbarnsdc#FactorAnalysis
:FactorAnalysis rdf:type owl:Class ;
                rdfs:subClassOf :CalculatedRatios ;
                rdfs:isDefinedBy "https://www.w3id.org/statbarnsdc" ;
                skos:definition "A statistical method used to identify underlying latent factors that explain the patterns of correlations among observed variables." ;
                skos:prefLabel "FactorAnalysis" .


###  https://www.w3id.org/statbarnsdc#FreqeuncyTable
:FreqeuncyTable rdf:type owl:Class ;
                rdfs:subClassOf :Frequencies ;
                rdfs:isDefinedBy "https://www.w3id.org/statbarnsdc" ;
                skos:definition "This class covers frequencies, i.e, counts of things, either in tables (most common), in certain graphs such as histograms or bar charts, or single as in a description of the number of survey participants. This also includes frequencies expressed as a proportion of some total." ;
                skos:prefLabel "FreqeuncyTable" .


###  https://www.w3id.org/statbarnsdc#Frequencies
:Frequencies rdf:type owl:Class ;
             rdfs:subClassOf :Statbarn ,
                             [ rdf:type owl:Restriction ;
                               owl:onProperty dpv-owl:hasRisk ;
                               owl:someValuesFrom :ClassDisclosure
                             ] ,
                             [ rdf:type owl:Restriction ;
                               owl:onProperty dpv-owl:hasRisk ;
                               owl:someValuesFrom :Differencing
                             ] ,
                             [ rdf:type owl:Restriction ;
                               owl:onProperty dpv-owl:hasRisk ;
                               owl:someValuesFrom :LowCount
                             ] ;
             rdfs:isDefinedBy "https://www.w3id.org/statbarnsdc" ;
             skos:definition "This class covers frequencies ie counts of things, either in tables (most common), in certain graphs such as histograms or bar charts, or single as in a description of the number of survey participants. This also includes frequencies expressed as a proportion of some total." ;
             skos:prefLabel "Frequencies" .


###  https://www.w3id.org/statbarnsdc#FriedmanTest
:FriedmanTest rdf:type owl:Class ;
              rdfs:subClassOf :StatisticalHypothesisTests ;
              rdfs:isDefinedBy "https://www.w3id.org/statbarnsdc" ;
              skos:definition "Non-parametric statistical test used to detect differences in treatments across multiple related groups." ;
              skos:prefLabel "FriedmanTest" .


###  https://www.w3id.org/statbarnsdc#GeneralLinearModel
:GeneralLinearModel rdf:type owl:Class ;
                    rdfs:subClassOf :CorrelationCoefficients ;
                    rdfs:isDefinedBy "https://www.w3id.org/statbarnsdc" ;
                    skos:definition "Models a continuous outcome as a linear combination of predictor variables." ;
                    skos:prefLabel "GeneralLinearModel" .


###  https://www.w3id.org/statbarnsdc#GeographicalAggregation
:GeographicalAggregation rdf:type owl:Class ;
                         rdfs:subClassOf :Aggregation ;
                         rdfs:isDefinedBy "https://www.w3id.org/statbarnsdc" ;
                         skos:definition "Combining spatial or location-based data into larger geographic units to reduce disclosure risk" ;
                         skos:prefLabel "GeographicalAggregation" .


###  https://www.w3id.org/statbarnsdc#GiniCoefficient
:GiniCoefficient rdf:type owl:Class ;
                 rdfs:subClassOf :Statbarn ,
                                 [ rdf:type owl:Restriction ;
                                   owl:onProperty dpv-owl:hasRisk ;
                                   owl:someValuesFrom :LowCount
                                 ] ;
                 rdfs:isDefinedBy "https://www.w3id.org/statbarnsdc" ;
                 skos:definition "The Gini coefficient is used to summarise inequality within a population. The Lorenz curve is its graphical counterpart." ;
                 skos:prefLabel "GiniCoefficient" .


###  https://www.w3id.org/statbarnsdc#GiniCurves
:GiniCurves rdf:type owl:Class ;
            rdfs:subClassOf :GiniCoefficient ;
            rdfs:isDefinedBy "https://www.w3id.org/statbarnsdc" ;
            skos:definition "A graphical representation showing the cumulative proportion of the population against the cumulative proportion of the resource." ;
            skos:prefLabel "GiniCurves" .


###  https://www.w3id.org/statbarnsdc#HazardRatio
:HazardRatio rdf:type owl:Class ;
             rdfs:subClassOf :Frequencies ;
             rdfs:isDefinedBy "https://www.w3id.org/statbarnsdc" ;
             skos:definition "A measure used in survival analysis that compares the hazard (event rate) between two groups over time." ;
             skos:prefLabel "HazardRatio" .


###  https://www.w3id.org/statbarnsdc#HazardSurvivalTables
:HazardSurvivalTables rdf:type owl:Class ;
                      rdfs:subClassOf :Statbarn ,
                                      [ rdf:type owl:Restriction ;
                                        owl:onProperty dpv-owl:hasRisk ;
                                        owl:someValuesFrom :ImplicitTables
                                      ] ,
                                      [ rdf:type owl:Restriction ;
                                        owl:onProperty dpv-owl:hasRisk ;
                                        owl:someValuesFrom :LowDOF
                                      ] ;
                      rdfs:isDefinedBy "https://www.w3id.org/statbarnsdc" ;
                      skos:definition "These are tables used to analyse and model survival or failure times in event-based data and business data. Commonly seen in epidemiology, actuarial science and clinical research among others. These can also underpin visualisations such as Kaplen-Meier." ;
                      skos:prefLabel "HazardSurvivalTables" .


###  https://www.w3id.org/statbarnsdc#HazardTables
:HazardTables rdf:type owl:Class ;
              rdfs:subClassOf :HazardSurvivalTables ;
              rdfs:isDefinedBy "https://www.w3id.org/statbarnsdc" ;
              skos:definition "Tables that summarize the hazard (event) rates over time." ;
              skos:prefLabel "HazardTables" .


###  https://www.w3id.org/statbarnsdc#Heatmap
:Heatmap rdf:type owl:Class ;
         rdfs:subClassOf :Frequencies ;
         rdfs:isDefinedBy "https://www.w3id.org/statbarnsdc" ;
         skos:definition "A graphical representation of data where values are displayed as colors in a matrix or grid." ;
         skos:prefLabel "Heatmap" .


###  https://www.w3id.org/statbarnsdc#HerfindahlHirschmanIndex
:HerfindahlHirschmanIndex rdf:type owl:Class ;
                          rdfs:subClassOf :NonLinearConcentrationRatios ;
                          rdfs:isDefinedBy "https://www.w3id.org/statbarnsdc" ;
                          skos:definition "A measure of concentration calculated by summing the squares of the shares of all elements." ;
                          skos:prefLabel "HerfindahlHirschmanIndex" .


###  https://www.w3id.org/statbarnsdc#Histogram
:Histogram rdf:type owl:Class ;
           rdfs:subClassOf :Frequencies ;
           rdfs:isDefinedBy "https://www.w3id.org/statbarnsdc" ;
           skos:definition "A graphical representation of a dataset that displays the frequency of values within consecutive intervals." ;
           skos:prefLabel "Histogram" .


###  https://www.w3id.org/statbarnsdc#HomogeneityOfRegression
:HomogeneityOfRegression rdf:type owl:Class ;
                         rdfs:subClassOf :StatisticalHypothesisTests ;
                         rdfs:isDefinedBy "https://www.w3id.org/statbarnsdc" ;
                         skos:definition "An assumption in ANCOVA stating that the relationship (slope) between the covariate and the dependent variable is the same across all groups." ;
                         skos:prefLabel "HomogeneityOfRegression" .


###  https://www.w3id.org/statbarnsdc#HomogeneityOfVariance
:HomogeneityOfVariance rdf:type owl:Class ;
                       rdfs:subClassOf :StatisticalHypothesisTests ;
                       rdfs:isDefinedBy "https://www.w3id.org/statbarnsdc" ;
                       skos:definition "An assumption in statistical tests (like ANOVA) that the variances of the dependent variable are equal across all groups or samples being compared." ;
                       skos:prefLabel "HomogeneityOfVariance" .


###  https://www.w3id.org/statbarnsdc#HomogeneityOfVarianceCovarianceMatrices
:HomogeneityOfVarianceCovarianceMatrices rdf:type owl:Class ;
                                         rdfs:subClassOf :StatisticalHypothesisTests ;
                                         rdfs:isDefinedBy "https://www.w3id.org/statbarnsdc" ;
                                         skos:definition "An assumption in multivariate analyses (like MANOVA) that the variance and covariance structure of the dependent variables is equal across all groups." ;
                                         skos:prefLabel "HomogeneityOfVarianceCovarianceMatrices" .


###  https://www.w3id.org/statbarnsdc#HosmerLemeshowTest
:HosmerLemeshowTest rdf:type owl:Class ;
                    rdfs:subClassOf :StatisticalHypothesisTests ;
                    rdfs:isDefinedBy "https://www.w3id.org/statbarnsdc" ;
                    skos:definition "Statistical test used in logistic regression to assess the goodness-of-fit of the model by comparing observed and predicted event probabilities across subgroups." ;
                    skos:prefLabel "HosmerLemeshowTest" .


###  https://www.w3id.org/statbarnsdc#ImplicitTables
:ImplicitTables rdf:type owl:Class ;
                rdfs:subClassOf dpv-owl:Risk ,
                                [ rdf:type owl:Restriction ;
                                  owl:onProperty risk-owl:hasRiskEvaluation ;
                                  owl:someValuesFrom :StatbarnDataCheck
                                ] ,
                                [ rdf:type owl:Restriction ;
                                  owl:onProperty dpv-owl:hasLikelihood ;
                                  owl:allValuesFrom dpv-owl:Likelihood
                                ] ,
                                [ rdf:type owl:Restriction ;
                                  owl:onProperty dpv-owl:hasRiskLevel ;
                                  owl:allValuesFrom dpv-owl:RiskLevel
                                ] ;
                rdfs:isDefinedBy "https://www.w3id.org/statbarnsdc" ;
                skos:definition "A risk of tables or outputs that allow sensitive information to be inferred indirectly through calculations or combinations of published data." ;
                skos:prefLabel "ImplicitTables" .


###  https://www.w3id.org/statbarnsdc#IndependentTtests
:IndependentTtests rdf:type owl:Class ;
                   rdfs:subClassOf :StatisticalHypothesisTests ;
                   rdfs:isDefinedBy "https://www.w3id.org/statbarnsdc" ;
                   skos:definition "Statistical test used to compare the means of two independent groups to determine if there is a significant difference between them." ;
                   skos:prefLabel "IndependentTtests" .


###  https://www.w3id.org/statbarnsdc#InterquartileRange
:InterquartileRange rdf:type owl:Class ;
                    rdfs:subClassOf :Position ;
                    rdfs:isDefinedBy "https://www.w3id.org/statbarnsdc" ;
                    skos:definition "The range between the first quartile and third quartile of a dataset." ;
                    skos:prefLabel "InterquartileRange" .


###  https://www.w3id.org/statbarnsdc#KValue
:KValue rdf:type owl:Class ;
        rdfs:subClassOf risk-owl:RiskCriteria ,
                        [ rdf:type owl:Restriction ;
                          owl:onProperty :hasDecimalValue ;
                          owl:someValuesFrom xsd:decimal
                        ] ;
        rdfs:isDefinedBy "https://www.w3id.org/statbarnsdc" ;
        skos:definition "A threshold parameter used in the NK disclosure risk test to determine whether a small number of records dominate a cell’s contribution, indicating potential disclosure risk." ;
        skos:prefLabel "KValue" .


###  https://www.w3id.org/statbarnsdc#KaiserMeyerOlkinTest
:KaiserMeyerOlkinTest rdf:type owl:Class ;
                      rdfs:subClassOf :StatisticalHypothesisTests ;
                      rdfs:isDefinedBy "https://www.w3id.org/statbarnsdc" ;
                      skos:definition "A measure of sampling adequacy for factor analysis, indicating whether the data are suitable for detecting underlying factors." ;
                      skos:prefLabel "KaiserMeyerOlkinTest" .


###  https://www.w3id.org/statbarnsdc#KaplanMeier
:KaplanMeier rdf:type owl:Class ;
             rdfs:subClassOf :HazardSurvivalTables ;
             rdfs:isDefinedBy "https://www.w3id.org/statbarnsdc" ;
             skos:definition "A statistical method used in survival analysis to estimate the probability of survival over time." ;
             skos:prefLabel "KaplanMeier" .


###  https://www.w3id.org/statbarnsdc#KappaMeasureOfAgreement
:KappaMeasureOfAgreement rdf:type owl:Class ;
                         rdfs:subClassOf :StatisticalHypothesisTests ;
                         rdfs:isDefinedBy "https://www.w3id.org/statbarnsdc" ;
                         skos:definition "A statistic that quantifies the agreement between two raters or observers for categorical data, adjusting for chance agreement." ;
                         skos:prefLabel "KappaMeasureOfAgreement" .


###  https://www.w3id.org/statbarnsdc#KendallsRank
:KendallsRank rdf:type owl:Class ;
              rdfs:subClassOf :CorrelationCoefficients ;
              rdfs:isDefinedBy "https://www.w3id.org/statbarnsdc" ;
              skos:definition "A measure of strength and direction of association between two ranked variables." ;
              skos:prefLabel "KendallsRank" .


###  https://www.w3id.org/statbarnsdc#KernelEstimates
:KernelEstimates rdf:type owl:Class ;
                 rdfs:subClassOf :CorrelationCoefficients ;
                 rdfs:isDefinedBy "https://www.w3id.org/statbarnsdc" ;
                 skos:definition "Estimate the probability density function or distribution." ;
                 skos:prefLabel "KernelEstimates" .


###  https://www.w3id.org/statbarnsdc#Kolmogorov-SmirnovTest
:Kolmogorov-SmirnovTest rdf:type owl:Class ;
                        rdfs:subClassOf :StatisticalHypothesisTests ;
                        rdfs:isDefinedBy "https://www.w3id.org/statbarnsdc" ;
                        skos:definition "A statistical test used to compare a sample distribution with a reference probability distribution or to compare two sample distributions, assessing whether they differ significantly." ;
                        skos:prefLabel "Kolmogorov-SmirnovTest" .


###  https://www.w3id.org/statbarnsdc#Kruskal-WallisTest
:Kruskal-WallisTest rdf:type owl:Class ;
                    rdfs:subClassOf :StatisticalHypothesisTests ;
                    rdfs:isDefinedBy "https://www.w3id.org/statbarnsdc" ;
                    skos:definition "A non-parametric statistical test used to compare the medians of three or more independent groups to determine if they come from the same distribution." ;
                    skos:prefLabel "Kruskal-WallisTest" .


###  https://www.w3id.org/statbarnsdc#Kurtosis
:Kurtosis rdf:type owl:Class ;
          rdfs:subClassOf :Shape ;
          rdfs:isDefinedBy "https://www.w3id.org/statbarnsdc" ;
          skos:definition "A statistical measure that describes the “tailedness” or peakedness of a data distribution." ;
          skos:prefLabel "Kurtosis" .


###  https://www.w3id.org/statbarnsdc#Lambda
:Lambda rdf:type owl:Class ;
        rdfs:subClassOf :StatisticalHypothesisTests ;
        rdfs:isDefinedBy "https://www.w3id.org/statbarnsdc" ;
        skos:definition "A measure of association for categorical variables, indicating the proportional reduction in error when predicting the dependent variable using the independent variable." ;
        skos:prefLabel "Lambda" .


###  https://www.w3id.org/statbarnsdc#LevenesTest
:LevenesTest rdf:type owl:Class ;
             rdfs:subClassOf :StatisticalHypothesisTests ;
             rdfs:isDefinedBy "https://www.w3id.org/statbarnsdc" ;
             skos:definition "A statistical test used to assess the equality of variances (homogeneity of variance) across two or more groups." ;
             skos:prefLabel "LevenesTest" .


###  https://www.w3id.org/statbarnsdc#LineGraph
:LineGraph rdf:type owl:Class ;
           rdfs:subClassOf :Frequencies ;
           rdfs:isDefinedBy "https://www.w3id.org/statbarnsdc" ;
           skos:definition "A chart that connects data points with lines to show trends, patterns, or changes of a variable over a continuous scale." ;
           skos:prefLabel "LineGraph" .


###  https://www.w3id.org/statbarnsdc#LinearAggregations
:LinearAggregations rdf:type owl:Class ;
                    rdfs:subClassOf :Statbarn ,
                                    [ rdf:type owl:Restriction ;
                                      owl:onProperty dpv-owl:hasRisk ;
                                      owl:someValuesFrom :Differencing
                                    ] ,
                                    [ rdf:type owl:Restriction ;
                                      owl:onProperty dpv-owl:hasRisk ;
                                      owl:someValuesFrom :Dominance
                                    ] ,
                                    [ rdf:type owl:Restriction ;
                                      owl:onProperty dpv-owl:hasRisk ;
                                      owl:someValuesFrom :LowCount
                                    ] ;
                    rdfs:isDefinedBy "https://www.w3id.org/statbarnsdc" ;
                    skos:definition "This class covers sums, means, ratios etc.  These are stats that provide a snapshot of the data's characteristics that don't relate to any one data point and instead are calculated with many or all of the points in a data set. This class also includes linear concentration ratios (eg share of the top N observations)." ;
                    skos:prefLabel "LinearAggregations" .


###  https://www.w3id.org/statbarnsdc#LinearRegressionCoefficients
:LinearRegressionCoefficients rdf:type owl:Class ;
                              rdfs:subClassOf :CorrelationCoefficients ;
                              rdfs:isDefinedBy "https://www.w3id.org/statbarnsdc" ;
                              skos:definition "Numerical values in a linear regression model that quantify the effect of each predictor variable on the outcome." ;
                              skos:prefLabel "LinearRegressionCoefficients" .


###  https://www.w3id.org/statbarnsdc#LinkedMultilevelTables
:LinkedMultilevelTables rdf:type owl:Class ;
                        rdfs:subClassOf :Statbarn ;
                        rdfs:isDefinedBy "https://www.w3id.org/statbarnsdc" ;
                        skos:definition "Multilevel and linked tables are used to summarize and analyze the relationship between multiple categorical variables. These often analyse nested categorical data in formats such as two or three way contingency tables or hierarchical contingency tables." ;
                        skos:prefLabel "LinkedMultilevelTables" .


###  https://www.w3id.org/statbarnsdc#LogLinearForHigherOrderTables
:LogLinearForHigherOrderTables rdf:type owl:Class ;
                               rdfs:subClassOf :CorrelationCoefficients ;
                               rdfs:isDefinedBy "https://www.w3id.org/statbarnsdc" ;
                               skos:definition "A statistical model used to analyze the relationships among three or more categorical variables." ;
                               skos:prefLabel "LogLinearForHigherOrderTables" .


###  https://www.w3id.org/statbarnsdc#LogisticRegression
:LogisticRegression rdf:type owl:Class ;
                    rdfs:subClassOf :CorrelationCoefficients ;
                    rdfs:isDefinedBy "https://www.w3id.org/statbarnsdc" ;
                    skos:definition "A statistical model used to predict the probability of a binary or categorical outcome." ;
                    skos:prefLabel "LogisticRegression" .


###  https://www.w3id.org/statbarnsdc#Logit
:Logit rdf:type owl:Class ;
       rdfs:subClassOf :CorrelationCoefficients ;
       rdfs:isDefinedBy "https://www.w3id.org/statbarnsdc" ;
       skos:definition "Used as the link function in logistic regression." ;
       skos:prefLabel "Logit" .


###  https://www.w3id.org/statbarnsdc#LongitudinalEstimation
:LongitudinalEstimation rdf:type owl:Class ;
                        rdfs:subClassOf :CorrelationCoefficients ;
                        rdfs:isDefinedBy "https://www.w3id.org/statbarnsdc" ;
                        skos:definition "A statistical method used to analyze data collected from the same subjects over time" ;
                        skos:prefLabel "LongitudinalEstimation" .


###  https://www.w3id.org/statbarnsdc#LowCount
:LowCount rdf:type owl:Class ;
          rdfs:subClassOf dpv-owl:Risk ,
                          [ rdf:type owl:Restriction ;
                            owl:onProperty risk-owl:hasRiskEvaluation ;
                            owl:someValuesFrom :MinimumThresholdCheck
                          ] ,
                          [ rdf:type owl:Restriction ;
                            owl:onProperty dpv-owl:hasLikelihood ;
                            owl:allValuesFrom dpv-owl:Likelihood
                          ] ,
                          [ rdf:type owl:Restriction ;
                            owl:onProperty dpv-owl:isMitigatedByMeasure ;
                            owl:allValuesFrom [ rdf:type owl:Class ;
                                                owl:unionOf ( :Noise
                                                              :Rounding
                                                              :Suppression
                                                            )
                                              ]
                          ] ;
          rdfs:isDefinedBy "https://www.w3id.org/statbarnsdc" ;
          skos:definition "The disclosure risk that arises when cells in a table have very few observations, making it easier to identify or infer information about the individuals contributing to those cells." ;
          skos:prefLabel "LowCount" .


###  https://www.w3id.org/statbarnsdc#LowDOF
:LowDOF rdf:type owl:Class ;
        rdfs:subClassOf dpv-owl:Risk ,
                        [ rdf:type owl:Restriction ;
                          owl:onProperty risk-owl:hasRiskEvaluation ;
                          owl:someValuesFrom :MinimumDoFCheck
                        ] ,
                        [ rdf:type owl:Restriction ;
                          owl:onProperty dpv-owl:hasLikelihood ;
                          owl:allValuesFrom dpv-owl:Likelihood
                        ] ,
                        [ rdf:type owl:Restriction ;
                          owl:onProperty dpv-owl:isMitigatedByMeasure ;
                          owl:allValuesFrom [ rdf:type owl:Class ;
                                              owl:unionOf ( :Aggregation
                                                            :Noise
                                                            :OutlierRemoval
                                                            :Suppression
                                                          )
                                            ]
                        ] ;
        rdfs:isDefinedBy "https://www.w3id.org/statbarnsdc" ;
        skos:definition "The risk that statistical outputs are based on very few independent pieces of information make it easier to deduce individual data or sensitive values." ;
        skos:prefLabel "LowDOF" .


###  https://www.w3id.org/statbarnsdc#MahalanobisDistance
:MahalanobisDistance rdf:type owl:Class ;
                     rdfs:subClassOf :Shape ;
                     rdfs:isDefinedBy "https://www.w3id.org/statbarnsdc" ;
                     skos:definition "A measure of the distance between a point and a distribution." ;
                     skos:prefLabel "MahalanobisDistance" .


###  https://www.w3id.org/statbarnsdc#Mancova
:Mancova rdf:type owl:Class ;
         rdfs:subClassOf :CorrelationCoefficients ;
         rdfs:isDefinedBy "https://www.w3id.org/statbarnsdc" ;
         skos:definition "A statistical technique that extends MANOVA by including covariates." ;
         skos:prefLabel "Mancova" .


###  https://www.w3id.org/statbarnsdc#MannWhitneyUTest
:MannWhitneyUTest rdf:type owl:Class ;
                  rdfs:subClassOf :StatisticalHypothesisTests ;
                  rdfs:isDefinedBy "https://www.w3id.org/statbarnsdc" ;
                  skos:definition "A non-parametric test used to compare differences between two independent groups on an ordinal or continuous outcome when the data do not assume a normal distribution." ;
                  skos:prefLabel "MannWhitneyUTest" .


###  https://www.w3id.org/statbarnsdc#MauchlySphericityTest
:MauchlySphericityTest rdf:type owl:Class ;
                       rdfs:subClassOf :StatisticalHypothesisTests ;
                       rdfs:isDefinedBy "https://www.w3id.org/statbarnsdc" ;
                       skos:definition "A statistical test used in repeated-measures ANOVA to assess whether the variances of the differences between all combinations of related groups are equal." ;
                       skos:prefLabel "MauchlySphericityTest" .


###  https://www.w3id.org/statbarnsdc#Maximum
:Maximum rdf:type owl:Class ;
         rdfs:subClassOf :Endpoints ;
         rdfs:isDefinedBy "https://www.w3id.org/statbarnsdc" ;
         skos:definition "The highest observed or recorded values of outcome." ;
         skos:prefLabel "Maximum" .


###  https://www.w3id.org/statbarnsdc#McNemarsTest
:McNemarsTest rdf:type owl:Class ;
              rdfs:subClassOf :StatisticalHypothesisTests ;
              rdfs:isDefinedBy "https://www.w3id.org/statbarnsdc" ;
              skos:definition "A statistical test used to analyze paired nominal data, typically to determine whether there is a significant change or difference in proportions for two related groups." ;
              skos:prefLabel "McNemarsTest" .


###  https://www.w3id.org/statbarnsdc#Mean
:Mean rdf:type owl:Class ;
      rdfs:subClassOf :LinearAggregations ;
      rdfs:isDefinedBy "https://www.w3id.org/statbarnsdc" ;
      skos:definition "The arithmetic average of a set of values, calculated by summing all values and dividing by their count." ;
      skos:prefLabel "Mean" .


###  https://www.w3id.org/statbarnsdc#MeanPlots
:MeanPlots rdf:type owl:Class ;
           rdfs:subClassOf :LinearAggregations ;
           rdfs:isDefinedBy "https://www.w3id.org/statbarnsdc" ;
           skos:definition "Graphs that display the average values of a variable for different groups or conditions." ;
           skos:prefLabel "MeanPlots" .


###  https://www.w3id.org/statbarnsdc#Median
:Median rdf:type owl:Class ;
        rdfs:subClassOf :Position ;
        rdfs:isDefinedBy "https://www.w3id.org/statbarnsdc" ;
        skos:definition "The middle value of a dataset when the values are arranged in order, dividing the data into two equal halves." ;
        skos:prefLabel "Median" .


###  https://www.w3id.org/statbarnsdc#Minimum
:Minimum rdf:type owl:Class ;
         rdfs:subClassOf :Endpoints ;
         rdfs:isDefinedBy "https://www.w3id.org/statbarnsdc" ;
         skos:definition "The lowest observed or recorded values of outcome." ;
         skos:prefLabel "Minimum" .


###  https://www.w3id.org/statbarnsdc#MinimumDOF
:MinimumDOF rdf:type owl:Class ;
            rdfs:subClassOf risk-owl:RiskCriteria ,
                            [ rdf:type owl:Restriction ;
                              owl:onProperty :hasDecimalValue ;
                              owl:someValuesFrom xsd:decimal
                            ] ;
            rdfs:isDefinedBy "https://www.w3id.org/statbarnsdc" ;
            skos:definition "The lowest acceptable number of 'residual degrees of freedom'  required for a statistical output to be considered safe from disclosure risk. Calculated as the number of independent data points minus the number of learned paramters in a model." ;
            skos:prefLabel "MinimumDOF" .


###  https://www.w3id.org/statbarnsdc#MinimumDoFCheck
:MinimumDoFCheck rdf:type owl:Class ;
                 rdfs:subClassOf risk-owl:RiskEvaluation ,
                                 [ rdf:type owl:Restriction ;
                                   owl:onProperty risk-owl:hasRiskCriteria ;
                                   owl:someValuesFrom :MinimumDOF
                                 ] ,
                                 [ rdf:type owl:Restriction ;
                                   owl:onProperty dpv-owl:hasHumanInvolvement ;
                                   owl:allValuesFrom dpv-owl:HumanInvolvement
                                 ] ;
                 rdfs:isDefinedBy "https://www.w3id.org/statbarnsdc" ;
                 skos:definition "To check model's residual degrees of Freedom (DoF) meets  or exceeds the specified value of MinimumDoF." ;
                 skos:prefLabel "MinimumDoFCheck" .


###  https://www.w3id.org/statbarnsdc#MinimumThreshold
:MinimumThreshold rdf:type owl:Class ;
                  rdfs:subClassOf risk-owl:RiskCriteria ,
                                  [ rdf:type owl:Restriction ;
                                    owl:onProperty :hasDecimalValue ;
                                    owl:someValuesFrom xsd:decimal
                                  ] ;
                  rdfs:isDefinedBy "https://www.w3id.org/statbarnsdc" ;
                  skos:definition "The smallest allowable value or count for a data cell or statistic to be safely released without risking disclosure of individual information." ;
                  skos:prefLabel "MinimumThreshold" .


###  https://www.w3id.org/statbarnsdc#MinimumThresholdCheck
:MinimumThresholdCheck rdf:type owl:Class ;
                       rdfs:subClassOf risk-owl:RiskEvaluation ,
                                       [ rdf:type owl:Restriction ;
                                         owl:onProperty risk-owl:hasRiskCriteria ;
                                         owl:someValuesFrom :MinimumThreshold
                                       ] ,
                                       [ rdf:type owl:Restriction ;
                                         owl:onProperty dpv-owl:hasHumanInvolvement ;
                                         owl:allValuesFrom dpv-owl:HumanInvolvement
                                       ] ;
                       rdfs:isDefinedBy "https://www.w3id.org/statbarnsdc" ;
                       skos:definition "To check the sizes if subgroups (e.g. table cells) meet or exceed the specified value of MinimumThreshold." ;
                       skos:prefLabel "MinimumThresholdCheck" .


###  https://www.w3id.org/statbarnsdc#Mode
:Mode rdf:type owl:Class ;
      rdfs:subClassOf :Statbarn ,
                      [ rdf:type owl:Restriction ;
                        owl:onProperty dpv-owl:hasRisk ;
                        owl:someValuesFrom :ClassDisclosure
                      ] ,
                      [ rdf:type owl:Restriction ;
                        owl:onProperty dpv-owl:hasRisk ;
                        owl:someValuesFrom :Differencing
                      ] ;
      rdfs:isDefinedBy "https://www.w3id.org/statbarnsdc" ;
      skos:definition "The value or values that occur most frequently in a dataset. It represents the peak or highest point on a distribution's histogram." ;
      skos:prefLabel "Mode" .


###  https://www.w3id.org/statbarnsdc#MultinomialLogit
:MultinomialLogit rdf:type owl:Class ;
                  rdfs:subClassOf :CorrelationCoefficients ;
                  rdfs:isDefinedBy "https://www.w3id.org/statbarnsdc" ;
                  skos:definition "A statistical model used to predict outcomes where the dependent variable has more than two discrete categories." ;
                  skos:prefLabel "MultinomialLogit" .


###  https://www.w3id.org/statbarnsdc#MultipleRegression
:MultipleRegression rdf:type owl:Class ;
                    rdfs:subClassOf :CorrelationCoefficients ;
                    rdfs:isDefinedBy "https://www.w3id.org/statbarnsdc" ;
                    skos:definition "A statistical method that models the relationship between one continuous dependent variable and two or more independent variables." ;
                    skos:prefLabel "MultipleRegression" .


###  https://www.w3id.org/statbarnsdc#MultipleRounding
:MultipleRounding rdf:type owl:Class ;
                  rdfs:subClassOf :Rounding ;
                  rdfs:isDefinedBy "https://www.w3id.org/statbarnsdc" ;
                  skos:definition "Values are rounded to the nearest multiple of a chosen base to reduce disclosure risk." ;
                  skos:prefLabel "MultipleRounding" .


###  https://www.w3id.org/statbarnsdc#MultiplicativeNoise
:MultiplicativeNoise rdf:type owl:Class ;
                     rdfs:subClassOf :Noise ;
                     rdfs:isDefinedBy "https://www.w3id.org/statbarnsdc" ;
                     skos:definition "Original data values are multiplied by random factors to mask individual contributions to reduce disclosure risk." ;
                     skos:prefLabel "MultiplicativeNoise" .


###  https://www.w3id.org/statbarnsdc#MultivariateAnalysisOfVariance
:MultivariateAnalysisOfVariance rdf:type owl:Class ;
                                rdfs:subClassOf :CorrelationCoefficients ;
                                rdfs:isDefinedBy "https://www.w3id.org/statbarnsdc" ;
                                skos:definition "Also reffered to as MANOVA, is a statistical technique that tests for differences across groups on two or more dependent variables simultaneously." ;
                                skos:prefLabel "MultivariateAnalysisOfVariance" .


###  https://www.w3id.org/statbarnsdc#NKCheck
:NKCheck rdf:type owl:Class ;
         rdfs:subClassOf risk-owl:RiskEvaluation ,
                         [ rdf:type owl:Restriction ;
                           owl:onProperty risk-owl:hasRiskCriteria ;
                           owl:someValuesFrom :KValue
                         ] ,
                         [ rdf:type owl:Restriction ;
                           owl:onProperty risk-owl:hasRiskCriteria ;
                           owl:someValuesFrom :NValue
                         ] ,
                         [ rdf:type owl:Restriction ;
                           owl:onProperty dpv-owl:hasHumanInvolvement ;
                           owl:allValuesFrom dpv-owl:HumanInvolvement
                         ] ;
         rdfs:isDefinedBy "https://www.w3id.org/statbarnsdc" ;
         skos:definition "NK test utilises the value specified as Nvalue and Kvalue." ;
         skos:prefLabel "NKCheck" .


###  https://www.w3id.org/statbarnsdc#NValue
:NValue rdf:type owl:Class ;
        rdfs:subClassOf risk-owl:RiskCriteria ,
                        [ rdf:type owl:Restriction ;
                          owl:onProperty :hasDecimalValue ;
                          owl:someValuesFrom xsd:decimal
                        ] ;
        rdfs:isDefinedBy "https://www.w3id.org/statbarnsdc" ;
        skos:definition "A threshold specifying the minimum number of observations required in a cell or output to ensure it meets disclosure control criteria." ;
        skos:prefLabel "NValue" .


###  https://www.w3id.org/statbarnsdc#NagelkerkeRSquared
:NagelkerkeRSquared rdf:type owl:Class ;
                    rdfs:subClassOf :StatisticalHypothesisTests ;
                    rdfs:isDefinedBy "https://www.w3id.org/statbarnsdc" ;
                    skos:definition "A pseudo R-squared measure for logistic regression." ;
                    skos:prefLabel "NagelkerkeRSquared" .


###  https://www.w3id.org/statbarnsdc#Noise
:Noise rdf:type owl:Class ;
       rdfs:subClassOf risk-owl:MitigationControl ;
       rdfs:isDefinedBy "https://www.w3id.org/statbarnsdc" ;
       skos:definition "Random or controlled perturbation added to data or outputs to mask individual contributions and reduce disclosure risk." ;
       skos:prefLabel "Noise" .


###  https://www.w3id.org/statbarnsdc#NonLinearConcentrationRatios
:NonLinearConcentrationRatios rdf:type owl:Class ;
                              rdfs:subClassOf :Statbarn ,
                                              [ rdf:type owl:Restriction ;
                                                owl:onProperty dpv-owl:hasRisk ;
                                                owl:someValuesFrom :Dominance
                                              ] ,
                                              [ rdf:type owl:Restriction ;
                                                owl:onProperty dpv-owl:hasRisk ;
                                                owl:someValuesFrom :LowCount
                                              ] ;
                              rdfs:isDefinedBy "https://www.w3id.org/statbarnsdc" ;
                              skos:definition "Non-linear concentration ratios are statistical measures used to assess degree of concentration or dispersion. The most common of these are the Herfindahl–Hirschman index." ;
                              skos:prefLabel "NonLinearConcentrationRatios" .


###  https://www.w3id.org/statbarnsdc#NumericalAggregation
:NumericalAggregation rdf:type owl:Class ;
                      rdfs:subClassOf :Aggregation ;
                      rdfs:isDefinedBy "https://www.w3id.org/statbarnsdc" ;
                      skos:definition "Summarizing or combining individual numerical values to reduce disclosure risk" ;
                      skos:prefLabel "NumericalAggregation" .


###  https://www.w3id.org/statbarnsdc#OddRatios
:OddRatios rdf:type owl:Class ;
           rdfs:subClassOf :CalculatedRatios ;
           rdfs:isDefinedBy "https://www.w3id.org/statbarnsdc" ;
           skos:definition "A measure of association that quantifies how the odds of an event occurring change with exposure to a predictor." ;
           skos:prefLabel "OddRatios" .


###  https://www.w3id.org/statbarnsdc#OmnibusTestsOfModelCoefficients
:OmnibusTestsOfModelCoefficients rdf:type owl:Class ;
                                 rdfs:subClassOf :CorrelationCoefficients ;
                                 rdfs:isDefinedBy "https://www.w3id.org/statbarnsdc" ;
                                 skos:definition "Statistical tests that assess whether a set of predictors, taken together, significantly improves the fit of a model compared to a null model with no predictors." ;
                                 skos:prefLabel "OmnibusTestsOfModelCoefficients" .


###  https://www.w3id.org/statbarnsdc#OutlierRemoval
:OutlierRemoval rdf:type owl:Class ;
                rdfs:subClassOf risk-owl:MitigationControl ;
                rdfs:isDefinedBy "https://www.w3id.org/statbarnsdc" ;
                skos:definition "Extreme or unusual values are removed or masked to prevent identification of individuals and reduce disclosure risk." ;
                skos:prefLabel "OutlierRemoval" .


###  https://www.w3id.org/statbarnsdc#PQCheck
:PQCheck rdf:type owl:Class ;
         rdfs:subClassOf risk-owl:RiskEvaluation ,
                         [ rdf:type owl:Restriction ;
                           owl:onProperty risk-owl:hasRiskCriteria ;
                           owl:someValuesFrom :PRatio
                         ] ,
                         [ rdf:type owl:Restriction ;
                           owl:onProperty dpv-owl:hasHumanInvolvement ;
                           owl:allValuesFrom dpv-owl:HumanInvolvement
                         ] ;
         rdfs:isDefinedBy "https://www.w3id.org/statbarnsdc" ;
         skos:definition "PQ test utilises the value specified as PRatio" ;
         skos:prefLabel "PQCheck" .


###  https://www.w3id.org/statbarnsdc#PRatio
:PRatio rdf:type owl:Class ;
        rdfs:subClassOf risk-owl:RiskCriteria ,
                        [ rdf:type owl:Restriction ;
                          owl:onProperty :hasDecimalValue ;
                          owl:someValuesFrom xsd:decimal
                        ] ;
        rdfs:isDefinedBy "https://www.w3id.org/statbarnsdc" ;
        skos:definition "A measure used to assess the proportion of a cell’s value contributed by a single or small group of individuals, indicating potential dominance and disclosure risk." ;
        skos:prefLabel "PRatio" .


###  https://www.w3id.org/statbarnsdc#PairedTtests
:PairedTtests rdf:type owl:Class ;
              rdfs:subClassOf :StatisticalHypothesisTests ;
              rdfs:isDefinedBy "https://www.w3id.org/statbarnsdc" ;
              skos:definition "Statistical test used to compare the means of two related or matched groups to determine if there is a significant difference between them." ;
              skos:prefLabel "PairedTtests" .


###  https://www.w3id.org/statbarnsdc#PanelDataModels
:PanelDataModels rdf:type owl:Class ;
                 rdfs:subClassOf :CorrelationCoefficients ;
                 rdfs:isDefinedBy "https://www.w3id.org/statbarnsdc" ;
                 skos:definition "Statistical models designed to analyze data that follow the same units over time for both cross-sectional and time-series variation." ;
                 skos:prefLabel "PanelDataModels" .


###  https://www.w3id.org/statbarnsdc#ParallelAnalysis
:ParallelAnalysis rdf:type owl:Class ;
                  rdfs:subClassOf :StatisticalHypothesisTests ;
                  rdfs:isDefinedBy "https://www.w3id.org/statbarnsdc" ;
                  skos:definition "A technique in factor analysis or principal component analysis used to determine the number of factors or components to retain by comparing the observed eigenvalues with those obtained from randomly generated data." ;
                  skos:prefLabel "ParallelAnalysis" .


###  https://www.w3id.org/statbarnsdc#PartialCorrelationCoefficients
:PartialCorrelationCoefficients rdf:type owl:Class ;
                                rdfs:subClassOf :CorrelationCoefficients ;
                                rdfs:isDefinedBy "https://www.w3id.org/statbarnsdc" ;
                                skos:definition "Measures the relationship between two variables while controlling the effect of one or more additional variables." ;
                                skos:prefLabel "PartialCorrelationCoefficients" .


###  https://www.w3id.org/statbarnsdc#PartialEtaSquared
:PartialEtaSquared rdf:type owl:Class ;
                   rdfs:subClassOf :StatisticalHypothesisTests ;
                   rdfs:isDefinedBy "https://www.w3id.org/statbarnsdc" ;
                   skos:definition "A measure of effect size in ANOVA that indicates the proportion of variance in the dependent variable explained by an independent variable, after controlling for other variables." ;
                   skos:prefLabel "PartialEtaSquared" .


###  https://www.w3id.org/statbarnsdc#PearsonsProductMomentCorrelationCoefficient
:PearsonsProductMomentCorrelationCoefficient rdf:type owl:Class ;
                                             rdfs:subClassOf :StatisticalHypothesisTests ;
                                             rdfs:isDefinedBy "https://www.w3id.org/statbarnsdc" ;
                                             skos:definition "Statistic that measures the strength and direction of the linear relationship between two continuous variables." ;
                                             skos:prefLabel "PearsonsProductMomentCorrelationCoefficient" .


###  https://www.w3id.org/statbarnsdc#PearsonsR
:PearsonsR rdf:type owl:Class ;
           rdfs:subClassOf :StatisticalHypothesisTests ;
           rdfs:isDefinedBy "https://www.w3id.org/statbarnsdc" ;
           skos:definition "A statistic that quantifies the strength and direction of the linear relationship between two continuous variables." ;
           skos:prefLabel "PearsonsR" .


###  https://www.w3id.org/statbarnsdc#PhiCoefficient
:PhiCoefficient rdf:type owl:Class ;
                rdfs:subClassOf :CorrelationCoefficients ;
                rdfs:isDefinedBy "https://www.w3id.org/statbarnsdc" ;
                skos:definition "A measure of association between two binary variables." ;
                skos:prefLabel "PhiCoefficient" .


###  https://www.w3id.org/statbarnsdc#PieChart
:PieChart rdf:type owl:Class ;
          rdfs:subClassOf :Frequencies ;
          rdfs:isDefinedBy "https://www.w3id.org/statbarnsdc" ;
          skos:definition "A circular chart that represents proportions of a whole by dividing the circle into slices corresponding to the relative sizes of categories." ;
          skos:prefLabel "PieChart" .


###  https://www.w3id.org/statbarnsdc#Position
:Position rdf:type owl:Class ;
          rdfs:subClassOf :Statbarn ,
                          [ rdf:type owl:Restriction ;
                            owl:onProperty dpv-owl:hasRisk ;
                            owl:someValuesFrom :ClassDisclosure
                          ] ,
                          [ rdf:type owl:Restriction ;
                            owl:onProperty dpv-owl:hasRisk ;
                            owl:someValuesFrom :LowCount
                          ] ;
          rdfs:isDefinedBy "https://www.w3id.org/statbarnsdc" ;
          skos:definition "Position refers to a statistic that provides information on a central or typical value in a dataset. These include data points such as median, percentiles, or inter-quartile range." ;
          skos:prefLabel "Position" .


###  https://www.w3id.org/statbarnsdc#PresenceOfLinkedTableCheck
:PresenceOfLinkedTableCheck rdf:type owl:Class ;
                            rdfs:subClassOf risk-owl:RiskEvaluation ,
                                            [ rdf:type owl:Restriction ;
                                              owl:onProperty risk-owl:hasRiskCriteria ;
                                              owl:someValuesFrom :PresenceOfLinkedTables
                                            ] ,
                                            [ rdf:type owl:Restriction ;
                                              owl:onProperty dpv-owl:hasHumanInvolvement ;
                                              owl:allValuesFrom dpv-owl:HumanInvolvement
                                            ] ;
                            rdfs:isDefinedBy "https://www.w3id.org/statbarnsdc" ;
                            skos:definition "To check for presence of linked tables and utilises value from PresenceOfLinkedTables. This will typically be a manual process" ;
                            skos:prefLabel "PresenceOfLinkedTableCheck" .


###  https://www.w3id.org/statbarnsdc#PresenceOfLinkedTables
:PresenceOfLinkedTables rdf:type owl:Class ;
                        rdfs:subClassOf risk-owl:RiskCriteria ,
                                        [ rdf:type owl:Restriction ;
                                          owl:onProperty :hasBooleanValue ;
                                          owl:someValuesFrom xsd:boolean
                                        ] ;
                        rdfs:isDefinedBy "https://www.w3id.org/statbarnsdc" ;
                        skos:definition "A measure specifying if there is a possibility that sensitive information can be inferred by combining multiple related tables, even if each table alone does not disclose individual data." ;
                        skos:prefLabel "PresenceOfLinkedTables" .


###  https://www.w3id.org/statbarnsdc#PresenceOfZero
:PresenceOfZero rdf:type owl:Class ;
                rdfs:subClassOf risk-owl:RiskCriteria ,
                                [ rdf:type owl:Restriction ;
                                  owl:onProperty :hasBooleanValue ;
                                  owl:someValuesFrom xsd:boolean
                                ] ;
                rdfs:isDefinedBy "https://www.w3id.org/statbarnsdc" ;
                skos:definition "A mesure specifying there are cells with a value of zero, which can reveal information about the absence of certain individuals or events." ;
                skos:prefLabel "PresenceOfZero" .


###  https://www.w3id.org/statbarnsdc#PresenceOfZeroCheck
:PresenceOfZeroCheck rdf:type owl:Class ;
                     rdfs:subClassOf risk-owl:RiskEvaluation ,
                                     [ rdf:type owl:Restriction ;
                                       owl:onProperty risk-owl:hasRiskCriteria ;
                                       owl:someValuesFrom :PresenceOfZero
                                     ] ,
                                     [ rdf:type owl:Restriction ;
                                       owl:onProperty dpv-owl:hasHumanInvolvement ;
                                       owl:allValuesFrom dpv-owl:HumanInvolvement
                                     ] ;
                     rdfs:isDefinedBy "https://www.w3id.org/statbarnsdc" ;
                     skos:definition "To check for presence of zeros and utilises value from PresenceOfZero." ;
                     skos:prefLabel "PresenceOfZeroCheck" .


###  https://www.w3id.org/statbarnsdc#PrevalenceRatio
:PrevalenceRatio rdf:type owl:Class ;
                 rdfs:subClassOf :Frequencies ;
                 rdfs:isDefinedBy "https://www.w3id.org/statbarnsdc" ;
                 skos:definition "A measure that compares the proportion of individuals with a condition in an exposed group to that in an unexposed group." ;
                 skos:prefLabel "PrevalenceRatio" .


###  https://www.w3id.org/statbarnsdc#PrimarySuppression
:PrimarySuppression rdf:type owl:Class ;
                    rdfs:subClassOf :Suppression ;
                    rdfs:isDefinedBy "https://www.w3id.org/statbarnsdc" ;
                    skos:definition "Masking of cells containing sensitive or high-risk values in a table to prevent disclosure." ;
                    skos:prefLabel "PrimarySuppression" .


###  https://www.w3id.org/statbarnsdc#PrincipalComponentAnalysis
:PrincipalComponentAnalysis rdf:type owl:Class ;
                            rdfs:subClassOf :StatisticalHypothesisTests ;
                            rdfs:isDefinedBy "https://www.w3id.org/statbarnsdc" ;
                            skos:definition "A dimensionality reduction technique that transforms correlated variables into a smaller set of uncorrelated components while retaining most of the original variance." ;
                            skos:prefLabel "PrincipalComponentAnalysis" .


###  https://www.w3id.org/statbarnsdc#Probit
:Probit rdf:type owl:Class ;
        rdfs:subClassOf :CorrelationCoefficients ;
        rdfs:isDefinedBy "https://www.w3id.org/statbarnsdc" ;
        skos:definition "A regression model used to predict the probability of a binary outcome by applying the inverse standard normal cumulative distribution function." ;
        skos:prefLabel "Probit" .


###  https://www.w3id.org/statbarnsdc#PseudoRSquared
:PseudoRSquared rdf:type owl:Class ;
                rdfs:subClassOf :StatisticalHypothesisTests ;
                rdfs:isDefinedBy "https://www.w3id.org/statbarnsdc" ;
                skos:definition "Measure used in models like logistic regression to indicate the proportion of variation in the dependent variable explained by the model." ;
                skos:prefLabel "PseudoRSquared" .


###  https://www.w3id.org/statbarnsdc#Quartiles
:Quartiles rdf:type owl:Class ;
           rdfs:subClassOf :Position ;
           rdfs:isDefinedBy "https://www.w3id.org/statbarnsdc" ;
           skos:definition "Values that divide a dataset into four equal parts." ;
           skos:prefLabel "Quartiles" .


###  https://www.w3id.org/statbarnsdc#RSquared
:RSquared rdf:type owl:Class ;
          rdfs:subClassOf :StatisticalHypothesisTests ;
          rdfs:isDefinedBy "https://www.w3id.org/statbarnsdc" ;
          skos:definition "Statistical measure that indicates the proportion of variance in the dependent variable explained by the independent variable(s) in a regression model." ;
          skos:prefLabel "RSquared" .


###  https://www.w3id.org/statbarnsdc#Range
:Range rdf:type owl:Class ;
       rdfs:subClassOf :Endpoints ;
       rdfs:isDefinedBy "https://www.w3id.org/statbarnsdc" ;
       skos:definition "The difference between the maximum and minimum values of a dataset, summarising the dispersion of the data." ;
       skos:prefLabel "Range" .


###  https://www.w3id.org/statbarnsdc#RequiredZeroCheck
:RequiredZeroCheck rdf:type owl:Class ;
                   rdfs:subClassOf risk-owl:RiskEvaluation ,
                                   [ rdf:type owl:Restriction ;
                                     owl:onProperty risk-owl:hasRiskCriteria ;
                                     owl:someValuesFrom :ZeroCheckDecider
                                   ] ,
                                   [ rdf:type owl:Restriction ;
                                     owl:onProperty dpv-owl:hasHumanInvolvement ;
                                     owl:allValuesFrom dpv-owl:HumanInvolvement
                                   ] ;
                   rdfs:isDefinedBy "https://www.w3id.org/statbarnsdc" ;
                   skos:definition "Indicates if a zerocheck is required and utilises the value from ZeroCheckDecider." ;
                   skos:prefLabel "RequiredZeroCheck" .


###  https://www.w3id.org/statbarnsdc#RiskRatios
:RiskRatios rdf:type owl:Class ;
            rdfs:subClassOf :CalculatedRatios ;
            rdfs:isDefinedBy "https://www.w3id.org/statbarnsdc" ;
            skos:definition "A measure that compares the probability of an event occurring in an exposed group to the probability in an unexposed group." ;
            skos:prefLabel "RiskRatios" .


###  https://www.w3id.org/statbarnsdc#Rounding
:Rounding rdf:type owl:Class ;
          rdfs:subClassOf risk-owl:MitigationControl ;
          rdfs:isDefinedBy "https://www.w3id.org/statbarnsdc" ;
          skos:definition "Numerical values are rounded to a specified precision to reduce the risk." ;
          skos:prefLabel "Rounding" .


###  https://www.w3id.org/statbarnsdc#ScatterGraph
:ScatterGraph rdf:type owl:Class ;
              rdfs:subClassOf :Frequencies ;
              rdfs:isDefinedBy "https://www.w3id.org/statbarnsdc" ;
              skos:definition "Also reffered to as scatter plot, a chart that displays individual data points on a two-dimensional plane, showing the relationship or correlation between two continuous variables." ;
              skos:prefLabel "ScatterGraph" .


###  https://www.w3id.org/statbarnsdc#SecondarySuppression
:SecondarySuppression rdf:type owl:Class ;
                      rdfs:subClassOf :Suppression ;
                      rdfs:isDefinedBy "https://www.w3id.org/statbarnsdc" ;
                      skos:definition "The additional suppression of non-sensitive cells in a table to prevent disclosure." ;
                      skos:prefLabel "SecondarySuppression" .


###  https://www.w3id.org/statbarnsdc#Shape
:Shape rdf:type owl:Class ;
       rdfs:subClassOf :Statbarn ,
                       [ rdf:type owl:Restriction ;
                         owl:onProperty dpv-owl:hasRisk ;
                         owl:someValuesFrom :LowDOF
                       ] ;
       rdfs:isDefinedBy "https://www.w3id.org/statbarnsdc" ;
       skos:definition "Shape outputs refer to measures that describe or show the characteristics of data distributions. They provide information on elements such as symmetry, peaks and tail behaviour. These comprise standard deviation, skewness, and kurtosis." ;
       skos:prefLabel "Shape" .


###  https://www.w3id.org/statbarnsdc#SimpleConcentrationRatio
:SimpleConcentrationRatio rdf:type owl:Class ;
                          rdfs:subClassOf :Frequencies ;
                          rdfs:isDefinedBy "https://www.w3id.org/statbarnsdc" ;
                          skos:definition "A measure that quantifies the dominance or contribution of the largest values or components in a dataset." ;
                          skos:prefLabel "SimpleConcentrationRatio" .


###  https://www.w3id.org/statbarnsdc#Skewness
:Skewness rdf:type owl:Class ;
          rdfs:subClassOf :Shape ;
          rdfs:isDefinedBy "https://www.w3id.org/statbarnsdc" ;
          skos:definition "A statistical measure that describes the asymmetry of a data distribution around its mean." ;
          skos:prefLabel "Skewness" .


###  https://www.w3id.org/statbarnsdc#SmoothedHistogram
:SmoothedHistogram rdf:type owl:Class ;
                   rdfs:subClassOf :Frequencies ;
                   rdfs:isDefinedBy "https://www.w3id.org/statbarnsdc" ;
                   skos:definition "A visualization of a dataset’s distribution where raw histogram counts are smoothed to show a continuous approximation of the underlying probability density." ;
                   skos:prefLabel "SmoothedHistogram" .


###  https://www.w3id.org/statbarnsdc#SpearmansRankCorrelationCoefficient
:SpearmansRankCorrelationCoefficient rdf:type owl:Class ;
                                     rdfs:subClassOf :StatisticalHypothesisTests ;
                                     rdfs:isDefinedBy "https://www.w3id.org/statbarnsdc" ;
                                     skos:definition "Non-parametric measure that assesses the strength and direction of the monotonic relationship between two ranked or ordinal variables." ;
                                     skos:prefLabel "SpearmansRankCorrelationCoefficient" .


###  https://www.w3id.org/statbarnsdc#StandardDeviation
:StandardDeviation rdf:type owl:Class ;
                   rdfs:subClassOf :Shape ;
                   rdfs:isDefinedBy "https://www.w3id.org/statbarnsdc" ;
                   skos:definition "A measure of how spread out or dispersed the values in a dataset are from the mean." ;
                   skos:prefLabel "StandardDeviation" .


###  https://www.w3id.org/statbarnsdc#StandardisedRegressionCoefficients
:StandardisedRegressionCoefficients rdf:type owl:Class ;
                                    rdfs:subClassOf :CorrelationCoefficients ;
                                    rdfs:isDefinedBy "https://www.w3id.org/statbarnsdc" ;
                                    skos:definition "Regression coefficients that have been rescaled to have unit variance, allowing the comparison of the relative strength of different predictors in a regression model." ;
                                    skos:prefLabel "StandardisedRegressionCoefficients" .


###  https://www.w3id.org/statbarnsdc#Statbarn
:Statbarn rdf:type owl:Class ;
          rdfs:isDefinedBy "https://www.w3id.org/statbarnsdc" ;
          skos:definition "The Statbarn taxonomy is a framework that classifies types of statisticalanalyses by their disclosure characteristics, including risk, exceptions, and mitigation measures for its use in output statistical disclosure control." ;
          skos:prefLabel "Statbarn" .


###  https://www.w3id.org/statbarnsdc#StatbarnDataCheck
:StatbarnDataCheck rdf:type owl:Class ;
                   rdfs:subClassOf risk-owl:RiskEvaluation ,
                                   [ rdf:type owl:Restriction ;
                                     owl:onProperty risk-owl:hasRiskCriteria ;
                                     owl:someValuesFrom :StatbarnRelevantShowData
                                   ] ,
                                   [ rdf:type owl:Restriction ;
                                     owl:onProperty dpv-owl:hasHumanInvolvement ;
                                     owl:allValuesFrom dpv-owl:HumanInvolvement
                                   ] ;
                   rdfs:isDefinedBy "https://www.w3id.org/statbarnsdc" ;
                   skos:definition " To check whether the data related to statbarn is disclosive and utilises value from StatbarnRelevantShowData." ;
                   skos:prefLabel "StatbarnDataCheck" .


###  https://www.w3id.org/statbarnsdc#StatbarnRelevantShowData
:StatbarnRelevantShowData rdf:type owl:Class ;
                          rdfs:subClassOf risk-owl:RiskCriteria ,
                                          [ rdf:type owl:Restriction ;
                                            owl:onProperty :hasBooleanValue ;
                                            owl:someValuesFrom xsd:boolean
                                          ] ;
                          rdfs:isDefinedBy "https://www.w3id.org/statbarnsdc" ;
                          skos:definition "A measure specifying there is relevant data or information that could be disclosive relevant to the statbarn." ;
                          skos:prefLabel "StatbarnRelevantShowData" .


###  https://www.w3id.org/statbarnsdc#StatisticalHypothesisTests
:StatisticalHypothesisTests rdf:type owl:Class ;
                            rdfs:subClassOf :Statbarn ,
                                            [ rdf:type owl:Restriction ;
                                              owl:onProperty dpv-owl:hasRisk ;
                                              owl:someValuesFrom :LowDOF
                                            ] ;
                            rdfs:isDefinedBy "https://www.w3id.org/statbarnsdc" ;
                            skos:definition "Statistical tests are used to make inferences and observe differences in data. These involve a wide range of tests including t-tests, p-values, F-tests, or confidence intervals." ;
                            skos:prefLabel "StatisticalHypothesisTests" .


###  https://www.w3id.org/statbarnsdc#StructuralEquationModelling
:StructuralEquationModelling rdf:type owl:Class ;
                             rdfs:subClassOf :CorrelationCoefficients ;
                             rdfs:isDefinedBy "https://www.w3id.org/statbarnsdc" ;
                             skos:definition "A multivariate statistical technique that analyzes complex relationships among observed and latent variables, combining factor analysis and multiple regression into a single model." ;
                             skos:prefLabel "StructuralEquationModelling" .


###  https://www.w3id.org/statbarnsdc#Sum
:Sum rdf:type owl:Class ;
     rdfs:subClassOf :LinearAggregations ;
     rdfs:isDefinedBy "https://www.w3id.org/statbarnsdc" ;
     skos:definition "The total obtained by adding together all the values." ;
     skos:prefLabel "Sum" .


###  https://www.w3id.org/statbarnsdc#Suppression
:Suppression rdf:type owl:Class ;
             rdfs:subClassOf risk-owl:MitigationControl ;
             rdfs:isDefinedBy "https://www.w3id.org/statbarnsdc" ;
             skos:definition "Sensitive cells or values are deliberately withheld or hidden to prevent disclosure risk." ;
             skos:prefLabel "Suppression" .


###  https://www.w3id.org/statbarnsdc#SurvivalTables
:SurvivalTables rdf:type owl:Class ;
                rdfs:subClassOf :HazardSurvivalTables ;
                rdfs:isDefinedBy "https://www.w3id.org/statbarnsdc" ;
                skos:definition "Tables that show the probability of survival at different time intervals" ;
                skos:prefLabel "SurvivalTables" .


###  https://www.w3id.org/statbarnsdc#TargetedNoise
:TargetedNoise rdf:type owl:Class ;
               rdfs:subClassOf :Noise ;
               rdfs:isDefinedBy "https://www.w3id.org/statbarnsdc" ;
               skos:definition "Noise is selectively added to specific high-risk values or records to reduce disclosure risk." ;
               skos:prefLabel "TargetedNoise" .


###  https://www.w3id.org/statbarnsdc#TemporalAggregation
:TemporalAggregation rdf:type owl:Class ;
                     rdfs:subClassOf :Aggregation ;
                     rdfs:isDefinedBy "https://www.w3id.org/statbarnsdc" ;
                     skos:definition "Combining data over time periods to reduce disclosure risk" ;
                     skos:prefLabel "TemporalAggregation" .


###  https://www.w3id.org/statbarnsdc#ThreeStageLeastSquares
:ThreeStageLeastSquares rdf:type owl:Class ;
                        rdfs:subClassOf :CorrelationCoefficients ;
                        rdfs:isDefinedBy "https://www.w3id.org/statbarnsdc" ;
                        skos:definition "An econometric method that estimates systems of simultaneous equations by combining Two-Stage Least Squares (2SLS) with seemingly unrelated regression." ;
                        skos:prefLabel "ThreeStageLeastSquares" .


###  https://www.w3id.org/statbarnsdc#TrimmedMean
:TrimmedMean rdf:type owl:Class ;
             rdfs:subClassOf :LinearAggregations ;
             rdfs:isDefinedBy "https://www.w3id.org/statbarnsdc" ;
             skos:definition "A measure of central tendency calculated by removing a specified percentage of the smallest and largest values from a dataset and then computing the mean of the remaining values." ;
             skos:prefLabel "TrimmedMean" .


###  https://www.w3id.org/statbarnsdc#TukeysHonestySignificantDifferenceTest
:TukeysHonestySignificantDifferenceTest rdf:type owl:Class ;
                                        rdfs:subClassOf :StatisticalHypothesisTests ;
                                        rdfs:isDefinedBy "https://www.w3id.org/statbarnsdc" ;
                                        skos:definition "A post-hoc analysis used after ANOVA to compare all possible pairs of group means and determine which differences are statistically significant." ;
                                        skos:prefLabel "TukeysHonestySignificantDifferenceTest" .


###  https://www.w3id.org/statbarnsdc#TwoStageLeastSquares
:TwoStageLeastSquares rdf:type owl:Class ;
                      rdfs:subClassOf :CorrelationCoefficients ;
                      rdfs:isDefinedBy "https://www.w3id.org/statbarnsdc" ;
                      skos:definition "An econometric method used to estimate parameters in simultaneous equations models." ;
                      skos:prefLabel "TwoStageLeastSquares" .


###  https://www.w3id.org/statbarnsdc#TwoWayAnalysisOfVariance
:TwoWayAnalysisOfVariance rdf:type owl:Class ;
                          rdfs:subClassOf :CorrelationCoefficients ;
                          rdfs:isDefinedBy "https://www.w3id.org/statbarnsdc" ;
                          skos:definition "Two-Way ANOVA is a statistical technique that examines the effect of two independent factors on a continuous dependent variable." ;
                          skos:prefLabel "TwoWayAnalysisOfVariance" .


###  https://www.w3id.org/statbarnsdc#VarianceCovarianceMatrix
:VarianceCovarianceMatrix rdf:type owl:Class ;
                          rdfs:subClassOf :Frequencies ;
                          rdfs:isDefinedBy "https://www.w3id.org/statbarnsdc" ;
                          skos:definition "A square matrix that displays the variances of variables along the diagonal and the covariances between variables in the off-diagonal elements." ;
                          skos:prefLabel "VarianceCovarianceMatrix" .


###  https://www.w3id.org/statbarnsdc#WaterfallChart
:WaterfallChart rdf:type owl:Class ;
                rdfs:subClassOf :Frequencies ;
                rdfs:isDefinedBy "https://www.w3id.org/statbarnsdc" ;
                skos:definition "A type of chart that visualizes how an initial value is affected by sequential positive and negative changes." ;
                skos:prefLabel "WaterfallChart" .


###  https://www.w3id.org/statbarnsdc#WilcoxonSignedRankTest
:WilcoxonSignedRankTest rdf:type owl:Class ;
                        rdfs:subClassOf :StatisticalHypothesisTests ;
                        rdfs:isDefinedBy "https://www.w3id.org/statbarnsdc" ;
                        skos:definition "A non-parametric test used to compare two related or paired samples to assess whether their population mean ranks differ, often as an alternative to the paired t-test when data are not normally distributed." ;
                        skos:prefLabel "WilcoxonSignedRankTest" .


###  https://www.w3id.org/statbarnsdc#WilksLambda
:WilksLambda rdf:type owl:Class ;
             rdfs:subClassOf :StatisticalHypothesisTests ;
             rdfs:isDefinedBy "https://www.w3id.org/statbarnsdc" ;
             skos:definition "A statistic used in multivariate analysis (like MANOVA) to test whether group means on a combination of dependent variables are equal, with smaller values indicating greater differences between groups." ;
             skos:prefLabel "WilksLambda" .


###  https://www.w3id.org/statbarnsdc#ZeroCheckDecider
:ZeroCheckDecider rdf:type owl:Class ;
                  rdfs:subClassOf risk-owl:RiskCriteria ,
                                  [ rdf:type owl:Restriction ;
                                    owl:onProperty :hasBooleanValue ;
                                    owl:someValuesFrom xsd:boolean
                                  ] ;
                  rdfs:isDefinedBy "https://www.w3id.org/statbarnsdc" ;
                  skos:definition "A measure that specifies if a zero check will be necessary for a TRE or any other organisation." ;
                  skos:prefLabel "ZeroCheckDecider" .


###  https://www.w3id.org/statbarnsdc#ZeroOrderCorrelation
:ZeroOrderCorrelation rdf:type owl:Class ;
                      rdfs:subClassOf :CorrelationCoefficients ;
                      rdfs:isDefinedBy "https://www.w3id.org/statbarnsdc" ;
                      skos:definition "A simple bivariate correlation between two variables" ;
                      skos:prefLabel "ZeroOrderCorrelation" .


#################################################################
#    General axioms
#################################################################

[ rdf:type owl:AllDisjointClasses ;
  owl:members ( :CalculatedRatios
                :Clusters
                :CorrelationCoefficients
                :Endpoints
                :Frequencies
                :GiniCoefficient
                :HazardSurvivalTables
                :LinearAggregations
                :LinkedMultilevelTables
                :Mode
                :NonLinearConcentrationRatios
                :Position
                :Shape
                :StatisticalHypothesisTests
              )
] .


[ rdf:type owl:AllDisjointClasses ;
  owl:members ( :KValue
                :MinimumDOF
                :MinimumThreshold
                :NValue
                :PRatio
                :PresenceOfLinkedTables
                :PresenceOfZero
                :StatbarnRelevantShowData
                :ZeroCheckDecider
              )
] .


###  Generated by the OWL API (version 4.5.29.2024-05-13T12:11:03Z) https://github.com/owlcs/owlapi
